finish dns example

src/BinEncoders/Env/BinLib/Core.v
@@ -7,5 +7,6 @@ Definition btransformer : Transformer :=
   {| bin := list bool;
      transform := @app _;
      transform_id := nil;
-     transform_id_pf := @app_nil_l _;
+     transform_id_left := @app_nil_l _;
+     transform_id_right := @app_nil_r _;
      transform_assoc := @app_assoc _ |}.
